src/tls/Handshake.fst
@@ -433,7 +433,7 @@ let client_handle_server_hello_done (HS #r0 #peer r res cfg id lgref hsref) msgs
        let ske_sig = ske.ske_sig in
        let cs_sigalg = Some.v n.n_sigAlg in
        let csr = (n.n_client_random @| n.n_server_random) in
-       if Cert.verify_signature c.crt_chain n.n_protocol_version cs_sigalg n.n_extensions.ne_signature_algorithms ske_tbs ske_sig then
+       if Cert.verify_signature c.crt_chain n.n_protocol_version csr cs_sigalg n.n_extensions.ne_signature_algorithms ske_tbs ske_sig then
          (match ske.ske_kex_s with
          | KEX_S_DHE gy ->
            let gx, pms = dh_shared_secret2 gy in
